Iris/Iris/HeapLang/Instances.lean
@@ -62,42 +62,42 @@ theorem mk_pure_prim_step {e1 e2 : Exp}
       have h := (EctxLanguage.baseStep_of_primStep Hstep hsub)
       apply hpure; apply h
 
-instance instPureExecIfTrue: Language.PureExec True 1 hl(if #true then ?e1 else ?e2) e1 where
+instance instPureExecIfTrue: Language.PureExec True 1 hl(if #true then &e1 else &e2) e1 where
   pureExec _ := Relation.Iterate.once <| mk_pure_prim_step (by intro; constructor) (by intro _ _ _ _ _ hs; cases hs; simp) <| by
     apply EctxItemLanguage.subredexes_are_values
     intro Ki e_inner heq
     cases Ki <;> cases heq
     simp [toVal]
 
-instance instPureExecIfFalse : Language.PureExec True 1 hl(if #false then ?e1 else ?e2) e2 where
+instance instPureExecIfFalse : Language.PureExec True 1 hl(if #false then &e1 else &e2) e2 where
   pureExec _ := Relation.Iterate.once <| mk_pure_prim_step (by intro; constructor) (by intro _ _ _ _ _ hs; cases hs; simp) <| by
     apply EctxItemLanguage.subredexes_are_values
     intro Ki e_inner heq
     cases Ki <;> cases heq
     simp [toVal]
 
-instance instPureExecCaseInjl {v e1 e2} : Language.PureExec True 1 (Exp.case hl(v(injl(?v))) e1 e2) (.app e1 (.ofVal v)) where
+instance instPureExecCaseInjl {v e1 e2} : Language.PureExec True 1 (Exp.case hl(v(injl(&v))) e1 e2) (.app e1 (.ofVal v)) where
   pureExec _ := Relation.Iterate.once <| mk_pure_prim_step (by intro; constructor) (by intro _ _ _ _ _ hs; cases hs; simp) <| by
     apply EctxItemLanguage.subredexes_are_values
     intro Ki e_inner heq
     cases Ki <;> cases heq
     simp [toVal]
 
-instance instPureExecCaseInjr {v e1 e2} : Language.PureExec True 1 (Exp.case hl(v(injr(?v))) e1 e2) (.app e2 (.ofVal v)) where
+instance instPureExecCaseInjr {v e1 e2} : Language.PureExec True 1 (Exp.case hl(v(injr(&v))) e1 e2) (.app e2 (.ofVal v)) where
   pureExec _ := Relation.Iterate.once <| mk_pure_prim_step (by intro; constructor) (by intro _ _ _ _ _ hs; cases hs; simp) <| by
     apply EctxItemLanguage.subredexes_are_values
     intro Ki e_inner heq
     cases Ki <;> cases heq
     simp [toVal]
 
-instance PureExec_injl {v : Val} : Language.PureExec True 1 hl(injl(?v)) hl(v(injl(?v)))  where
+instance PureExec_injl {v : Val} : Language.PureExec True 1 hl(injl(&v)) hl(v(injl(&v)))  where
   pureExec _ := Relation.Iterate.once <| mk_pure_prim_step (by intro; constructor) (by intro _ _ _ _ _ hs; cases hs; simp) <| by
     apply EctxItemLanguage.subredexes_are_values
     intro Ki e_inner heq
     cases Ki <;> cases heq
     simp [toVal]
 
-instance PureExec_injr {v : Val} : Language.PureExec True 1 hl(injr(?v)) hl(v(injr(?v)))  where
+instance PureExec_injr {v : Val} : Language.PureExec True 1 hl(injr(&v)) hl(v(injr(&v)))  where
   pureExec _ := Relation.Iterate.once <| mk_pure_prim_step (by intro; constructor) (by intro _ _ _ _ _ hs; cases hs; simp) <| by
     apply EctxItemLanguage.subredexes_are_values
     intro Ki e_inner heq
@@ -105,32 +105,32 @@ instance PureExec_injr {v : Val} : Language.PureExec True 1 hl(injr(?v)) hl(v(in
     simp [toVal]
 
 instance instPureExecBeta {f x : Binder} {e : Exp} {v : Val} :
-    Language.PureExec True 1 hl(v(rec ?f ?x := ?e) ?v) ((e.subst f (.rec_ f x e)).subst x v) where
+    Language.PureExec True 1 hl(v(rec &f &x := &e) &v) ((e.subst f (.rec_ f x e)).subst x v) where
   pureExec _ := Relation.Iterate.once <| mk_pure_prim_step (by intro; constructor; simp) (by intro _ _ _ _ _ hs; cases hs; simp [*]) <| by
     apply EctxItemLanguage.subredexes_are_values
     intro Ki e_inner heq
     cases Ki <;> cases heq <;> simp [toVal]
 
-instance instPureExecRec {f x e} : Language.PureExec True 1 hl(rec ?f ?x := ?e) hl(v(rec ?f ?x := ?e)) where
+instance instPureExecRec {f x e} : Language.PureExec True 1 hl(rec &f &x := &e) hl(v(rec &f &x := &e)) where
   pureExec _ := Relation.Iterate.once <| mk_pure_prim_step (by intro; constructor) (by intro _ _ _ _ _ hs; cases hs; simp [*]) <| by
     apply EctxItemLanguage.subredexes_are_values
     intro Ki e_inner heq
     cases Ki <;> cases heq <;> simp [toVal]
 
 
-instance PureExec_fst {v1 v2 : Val} : Language.PureExec True 1 hl(fst(v((?v1, ?v2)))) v1 where
+instance PureExec_fst {v1 v2 : Val} : Language.PureExec True 1 hl(fst(v((&v1, &v2)))) v1 where
   pureExec _ := Relation.Iterate.once <| mk_pure_prim_step (by intro; constructor) (by intro _ _ _ _ _ hs; cases hs; simp [*]) <| by
     apply EctxItemLanguage.subredexes_are_values
     intro Ki e_inner heq
     cases Ki <;> cases heq <;> simp [toVal]
 
-instance PureExec_snd {v1 v2 : Val} : Language.PureExec True 1 hl(snd(v((?v1, ?v2)))) v2 where
+instance PureExec_snd {v1 v2 : Val} : Language.PureExec True 1 hl(snd(v((&v1, &v2)))) v2 where
   pureExec _ := Relation.Iterate.once <| mk_pure_prim_step (by intro; constructor) (by intro _ _ _ _ _ hs; cases hs; simp [*]) <| by
     apply EctxItemLanguage.subredexes_are_values
     intro Ki e_inner heq
     cases Ki <;> cases heq <;> simp [toVal]
 
-instance PureExec_pair {v1 v2 : Val} : Language.PureExec True 1 hl((?v1, ?v2)) hl(v((?v1, ?v2)))  where
+instance PureExec_pair {v1 v2 : Val} : Language.PureExec True 1 hl((&v1, &v2)) hl(v((&v1, &v2)))  where
   pureExec _ := Relation.Iterate.once <| mk_pure_prim_step (by intro; constructor) (by intro _ _ _ _ _ hs; cases hs; simp [*]) <| by
     apply EctxItemLanguage.subredexes_are_values
     intro Ki e_inner heq
@@ -143,9 +143,9 @@ instance PureExec_le_int {n1 n2 : Int} : Language.PureExec True 1 hl(#(.int n1) 
     cases Ki <;> cases heq <;> simp [toVal]
 
 
-instance instAtomicStore {s} {v1 v2 : Val} : Language.Atomic s hl(?v1 ← ?v2) where
+instance instAtomicStore {s} {v1 v2 : Val} : Language.Atomic s hl(&v1 ← &v2) where
   atomic {σ obs e' σ' eₜ} Hstep := by
-    have hsr : EctxLanguage.SubredexesAreValues hl(?v1 ← ?v2) := by
+    have hsr : EctxLanguage.SubredexesAreValues hl(&v1 ← &v2) := by
       apply EctxItemLanguage.subredexes_are_values
       intro Ki e_inner heq
       cases Ki <;> try (cases heq; done)
@@ -154,9 +154,9 @@ instance instAtomicStore {s} {v1 v2 : Val} : Language.Atomic s hl(?v1 ← ?v2) w
     rename_i l v Heq
     cases s <;> simp [toVal, Language.val_irreducible]
 
-instance instAtomicSnd {s} {v1 : Val} : Language.Atomic s hl(snd(?v1)) where
+instance instAtomicSnd {s} {v1 : Val} : Language.Atomic s hl(snd(&v1)) where
   atomic {σ obs e' σ' eₜ} Hstep := by
-    have hsr : EctxLanguage.SubredexesAreValues hl(snd(?v1)) := by
+    have hsr : EctxLanguage.SubredexesAreValues hl(snd(&v1)) := by
       apply EctxItemLanguage.subredexes_are_values
       intro Ki e_inner heq
       cases Ki <;> try (cases heq; done)
@@ -164,9 +164,9 @@ instance instAtomicSnd {s} {v1 : Val} : Language.Atomic s hl(snd(?v1)) where
     cases (EctxLanguage.baseStep_of_primStep Hstep hsr)
     cases s <;> simp [toVal, Language.val_irreducible]
 
-instance instAtomicCmpXChg {s} {v1 v2 v3 : Val} : Language.Atomic s hl(cmpXchg(?v1, ?v2, ?v3)) where
+instance instAtomicCmpXChg {s} {v1 v2 v3 : Val} : Language.Atomic s hl(cmpXchg(&v1, &v2, &v3)) where
   atomic {σ obs e' σ' eₜ} Hstep := by
-    have hsr : EctxLanguage.SubredexesAreValues hl(cmpXchg(?v1, ?v2, ?v3)) := by
+    have hsr : EctxLanguage.SubredexesAreValues hl(cmpXchg(&v1, &v2, &v3)) := by
       apply EctxItemLanguage.subredexes_are_values
       intro Ki e_inner heq
       cases Ki <;> try (cases heq; done)
