Iris/Iris/HeapLang/Notation.lean
@@ -34,13 +34,13 @@ macro_rules
 /-- escaping -/
 syntax:max "{" term "}" : hl_binder
 /-- escaping identifiers -/
-syntax:max "?" ident : hl_binder
+syntax:max "&" ident : hl_binder
 syntax:max binderIdent : hl_binder
 
 /-- escaping -/
 syntax:max "{" term "}" : hl_val
 /-- escaping identifiers -/
-syntax:max "?" ident : hl_val
+syntax:max "&" ident : hl_val
 /-- embedding literals -/
 syntax:max "#" term:max : hl_val
 /-- pairs -/
@@ -61,7 +61,7 @@ syntax:max "v{" term "}" : hl_exp
 /-- escaping -/
 syntax:max "{" term "}" : hl_exp
 /-- escaping identifiers -/
-syntax:max "?" ident : hl_exp
+syntax:max "&" ident : hl_exp
 /-- embedding literals -/
 syntax:max "#" term:max : hl_exp
 /-- variables -/
@@ -80,11 +80,11 @@ syntax:70 hl_exp:71 " / " hl_exp:70 : hl_exp
 /-- modulo -/
 syntax:70 hl_exp:71 " % " hl_exp:70 : hl_exp
 /-- and -/
-syntax:60 hl_exp:61 " & " hl_exp:60 : hl_exp
+syntax:60 hl_exp:61 " &&& " hl_exp:60 : hl_exp
 /-- or -/
-syntax:55 hl_exp:56 " | " hl_exp:55 : hl_exp
+syntax:55 hl_exp:56 " ||| " hl_exp:55 : hl_exp
 /-- xor -/
-syntax:58 hl_exp:59 " ^ " hl_exp:58 : hl_exp
+syntax:58 hl_exp:59 " ^^^ " hl_exp:58 : hl_exp
 /-- shiftl -/
 syntax:75 hl_exp:76 " <<< " hl_exp:75 : hl_exp
 /-- shiftr -/
@@ -140,9 +140,9 @@ syntax:100 "none()" : hl_exp
 syntax:100 "some(" hl_exp ")" : hl_exp
 
 /-- match -/
-syntax:100 "match " hl_exp:80 " with"
-  " | " hl_match_arm " => " hl_exp:80
-  " | " hl_match_arm " => " hl_exp:80 : hl_exp
+syntax:100 "match " hl_exp:5 " with"
+  " | " hl_match_arm " => " hl_exp:5
+  " | " hl_match_arm " => " hl_exp:5 : hl_exp
 
 syntax "injl(" hl_binder ")" : hl_match_arm
 syntax "injr(" hl_binder ")" : hl_match_arm
@@ -177,29 +177,29 @@ def hl_exp.parenthesizer : CategoryParenthesizer := fun prec => do
 
 partial def unpackHLExp [Monad m] [MonadRef m] [MonadQuotation m] : Term → m (TSyntax `hl_exp)
   | `(hl($e)) => `(hl_exp|$e)
-  | `($i:ident) => `(hl_exp|?$i)
+  | `($i:ident) => `(hl_exp|&$i)
   | `($t) => `(hl_exp|{$t})
 
 partial def unpackHLVal [Monad m] [MonadRef m] [MonadQuotation m] : Term → m (TSyntax `hl_val)
   | `(hl_val($e)) => `(hl_val|$e)
-  | `($i:ident) => `(hl_val|?$i)
+  | `($i:ident) => `(hl_val|&$i)
   | `($t) => `(hl_val|{$t})
 
 partial def unpackHLBinder [Monad m] [MonadRef m] [MonadQuotation m] : Term → m (TSyntax `hl_binder)
   | `(hl_binder($e)) => `(hl_binder|$e)
-  | `($i:ident) => `(hl_binder|?$i)
+  | `($i:ident) => `(hl_binder|&$i)
   | `($t) => `(hl_binder|{$t})
 
 /-- elaborating binders -/
 macro_rules
   | `(hl_binder(_)) => `(Binder.anon)
   | `(hl_binder($i:ident)) => `(Binder.named $(Syntax.mkStrLit i.getId.toString))
-  | `(hl_binder(?$i)) => `($i)
+  | `(hl_binder(&$i)) => `($i)
   | `(hl_binder({$t})) => `($t)
 
 /-- elaborating values -/
 macro_rules
-  | `(hl_val(? $i)) => pure i
+  | `(hl_val(& $i)) => pure i
   | `(hl_val({$t})) => pure t
   | `(hl_val(# $e)) => `(Val.lit $e)
   | `(hl_val(rec $f $x := $e)) => do `(Val.rec_ hl_binder($f) hl_binder($x) hl($e))
@@ -217,7 +217,7 @@ macro_rules
   | `(hl(($e))) => `(hl($e))
   | `(hl(_)) => `(_)
   | `(hl({$t})) => pure t
-  | `(hl(?$i)) => pure i
+  | `(hl(&$i)) => pure i
   | `(hl(v($e))) => `(@ToVal.ofVal Exp Val instToVal hl_val($e))
   | `(hl(v{$e})) => `(hl(v({$e})))
   | `(hl(# $e)) => `(hl(v(# $e)))
@@ -228,9 +228,9 @@ macro_rules
   | `(hl($e1 * $e2)) => `(Exp.binop BinOp.mult hl($e1) hl($e2))
   | `(hl($e1 / $e2)) => `(Exp.binop BinOp.tdiv hl($e1) hl($e2))
   | `(hl($e1 % $e2)) => `(Exp.binop BinOp.tmod hl($e1) hl($e2))
-  | `(hl($e1 & $e2)) => `(Exp.binop BinOp.and hl($e1) hl($e2))
-  | `(hl($e1 | $e2)) => `(Exp.binop BinOp.or hl($e1) hl($e2))
-  | `(hl($e1 ^ $e2)) => `(Exp.binop BinOp.xor hl($e1) hl($e2))
+  | `(hl($e1 &&& $e2)) => `(Exp.binop BinOp.and hl($e1) hl($e2))
+  | `(hl($e1 ||| $e2)) => `(Exp.binop BinOp.or hl($e1) hl($e2))
+  | `(hl($e1 ^^^ $e2)) => `(Exp.binop BinOp.xor hl($e1) hl($e2))
   | `(hl($e1 <<< $e2)) => `(Exp.binop BinOp.shiftl hl($e1) hl($e2))
   | `(hl($e1 >>> $e2)) => `(Exp.binop BinOp.shiftr hl($e1) hl($e2))
   | `(hl($e1 <= $e2)) => `(hl($e1 ≤ $e2))
@@ -359,9 +359,9 @@ def unexpBinop : Unexpander
   | `($_ BinOp.mult $e1 $e2) => do `(hl(($(← unpackHLExp e1) * $(← unpackHLExp e2))))
   | `($_ BinOp.tdiv $e1 $e2) => do `(hl(($(← unpackHLExp e1) / $(← unpackHLExp e2))))
   | `($_ BinOp.tmod $e1 $e2) => do `(hl(($(← unpackHLExp e1) % $(← unpackHLExp e2))))
-  | `($_ BinOp.and $e1 $e2) => do `(hl(($(← unpackHLExp e1) & $(← unpackHLExp e2))))
-  | `($_ BinOp.or $e1 $e2) => do `(hl(($(← unpackHLExp e1) | $(← unpackHLExp e2))))
-  | `($_ BinOp.xor $e1 $e2) => do `(hl(($(← unpackHLExp e1) ^ $(← unpackHLExp e2))))
+  | `($_ BinOp.and $e1 $e2) => do `(hl(($(← unpackHLExp e1) &&& $(← unpackHLExp e2))))
+  | `($_ BinOp.or $e1 $e2) => do `(hl(($(← unpackHLExp e1) ||| $(← unpackHLExp e2))))
+  | `($_ BinOp.xor $e1 $e2) => do `(hl(($(← unpackHLExp e1) ^^^ $(← unpackHLExp e2))))
   | `($_ BinOp.shiftl $e1 $e2) => do `(hl(($(← unpackHLExp e1) <<< $(← unpackHLExp e2))))
   | `($_ BinOp.shiftr $e1 $e2) => do `(hl(($(← unpackHLExp e1) >>> $(← unpackHLExp e2))))
   | `($_ BinOp.le $e1 $e2) => do `(hl(($(← unpackHLExp e1) ≤ $(← unpackHLExp e2))))
